

# Math 342 Tutorial

July 9, 2025

**Question 1.** Show that if  $n = p_1^{2e_1+1} \cdots p_k^{2e_k+1} q_1^{2f_1} \cdots q_m^{2f_m}$ , and if  $r$  is an odd prime not dividing  $n$ , then

$$\left(\frac{n}{r}\right) = \left(\frac{p_1}{r}\right) \cdots \left(\frac{p_k}{r}\right).$$

Using the fact that the Legendre symbol is totally multiplicative, we see at once that

$$\left(\frac{n}{r}\right) = \prod_{i=1}^k \underbrace{\left(\frac{p_i}{r}\right)^{2e_i}}_{=1} \prod_{j=1}^m \underbrace{\left(\frac{q_j}{r}\right)^{2f_j}}_{=1} = \prod_{i=1}^k \left(\frac{p_i}{r}\right).$$

**Question 2.** Show that if  $p$  is odd prime that is  $3 \pmod{4}$ , then  $[(p-1)/2]! \equiv (-1)^t \pmod{p}$  where  $t$  is the number of nonquadratic residues in the range  $0$  to  $[p/2]$  inclusive.

In a similar manner as assignment 4 question 4, we see that  $((p-1)/2)!^2 \equiv -(p-1)! \equiv 1 \pmod{p}$  by an application of Wilson's Theorem. By Euler's Criterion, we see that  $((p-1)/2)!^{(p-1)/2} \equiv (1 | p)(2 | p) \cdots ((p-1)/2 | p) \equiv (-1)^t \pmod{p}$ . Since  $((p-1)/2)! \equiv \pm 1 \pmod{p}$ , and since  $(p-1)/2$  is odd, we're done.

**Question 3.** Let  $p$  be an odd prime. Prove the following identities. (a)  $\sum_{r=1}^{p-1} r(r | p) = 0$  if  $p \equiv 1 \pmod{4}$ . (b)  $\sum_{\substack{r=1 \\ (r|p)=1}}^{p-1} r = \frac{p(p-1)}{4}$  if  $p \equiv 1 \pmod{4}$ . (c)  $\sum_{r=1}^{p-1} r^2(r | p) = p \sum_{r=1}^{p-1} r(r | p)$  if  $p \equiv 3 \pmod{4}$ . (d)  $\sum_{r=1}^{p-1} r^3(r | p) = \frac{3}{2}p \sum_{r=1}^{p-1} r^2(r | p)$  if  $p \equiv 1 \pmod{4}$ . (e)  $\sum_{r=1}^{p-1} r^4(r | p) = 2p \sum_{r=1}^{p-1} r^3(r | p) - p^2 \sum_{r=1}^{p-1} r^2(r | p)$  if  $p \equiv 3 \pmod{4}$ .

(a) Observe that  $(r | p) = (-1)^{(p-1)/2} (p-r | r)$  (why?). Since  $p \equiv 1 \pmod{4}$ , we then have

$$\sum_{r=1}^{p-1} r(r | p) = \sum_{r=1}^{p-1} (p-r)(p-r | p) = \sum_{r=1}^{p-1} (p-r)(r | p) = p \sum_{r=1}^{p-1} (r | p) - \sum_{r=1}^{p-1} r(r | p) = - \sum_{r=1}^{p-1} r(r | p).$$

(b) Since  $p \equiv 1 \pmod{4}$ , we have

$$\sum_{\substack{r=1 \\ (r|p)=1}}^{p-1} r = \sum_{\substack{r=1 \\ (r|p)=1}}^{p-1} (p-r) = p \sum_{\substack{r=1 \\ (r|p)=1}}^{p-1} 1 - \sum_{\substack{r=1 \\ (r|p)=1}}^{p-1} r.$$

Solving for  $\sum_{r=1, (r|p)=1}^{p-1} r$ , and using the fact that there are  $(p-1)/2$  quadratic residues modulo  $p$ , we obtain the result.

(c) Since  $p \equiv 3 \pmod{4}$ , we have

$$\begin{aligned} \sum_{r=1}^{p-1} r^2(r | p) &= \sum_{r=1}^{p-1} (p-r)^2(p-r | p) = - \sum_{r=1}^{p-1} (p-r)^2(r | p) \\ &= -p^2 \sum_{r=1}^{p-1} (r | p) + 2p \sum_{r=1}^{p-1} r(r | p) - \sum_{r=1}^{p-1} r^2(r | p) = 2p \sum_{r=1}^{p-1} r(r | p) - \sum_{r=1}^{p-1} r^2(r | p) \end{aligned}$$

Solving for  $\sum_{r=1}^{p-1} r^2(r | p)$  gives the result.

(d) For  $p \equiv 1 \pmod{4}$ , we have that

$$\begin{aligned}\sum_{r=1}^{p-1} r^3(r|p) &= \sum_{r=1}^{p-1} (p-r)^3(p-r|p) = \sum_{r=1}^{p-1} (p-r)^3(r|p) \\ &= p^3 \sum_{r=1}^{p-1} (r|p) - 3p^2 \sum_{r=1}^{p-1} r(r|p) + 3p \sum_{r=1}^{p-1} r^2(r|p) - \sum_{r=1}^{p-1} r^3(r|p).\end{aligned}$$

But  $\sum_{r=1}^{p-1} (r|p) = 0$ , and  $\sum_{r=1}^{p-1} r(r|p) = 0$  by part (a). Hence, we obtain the result by solving for  $\sum_{r=1}^{p-1} r^3(r|p)$ .

(e) Since  $p \equiv 3 \pmod{4}$ , we have

$$\begin{aligned}\sum_{r=1}^{p-1} r^4(r|p) &= \sum_{r=1}^{p-1} (p-r)^4(p-r|p) = - \sum_{r=1}^{p-1} (p-r)^4(r|p) \\ &= \sum_{i=0}^4 (-1)^{i+1} \binom{4}{i} p^{4-j} \sum_{r=1}^{p-1} r^i(r|p).\end{aligned}$$

From part (c), we know that  $p \sum_{r=1}^{p-1} r(r|p) = \sum_{r=1}^{p-1} r^2(r|p)$ . Substituting and solving, we obtain the result.

**Question 4.** Show that if  $a$  is a quadratic residue of the prime  $p$ , then the solutions of  $x^2 \equiv a \pmod{p}$  are (a)  $x \equiv \pm a^{n+1} \pmod{p}$  if  $p = 4n + 3$ , or (b)  $x \equiv \pm a^{n+1}$  or  $\pm 2^{2n+1} a^{n+1} \pmod{p}$  if  $p = 8n + 5$ .

(a) Since  $p = 4n + 3$ , we have that

$$x^2 \equiv (\pm a^{n+1})^2 \equiv a^{(p+1)/2} \equiv a^{(p-1)/2} a \equiv a \pmod{p}.$$

Hence, the solutions in this case are  $\pm a^{n+1} \pmod{p}$ .

(b) Because  $p \equiv 5 \pmod{8}$ , we know that  $-1$  is a quadratic residue and  $2$  is a quadratic non-residue modulo  $p$ . Next, observe that  $(\pm a^{n+1})^2 \equiv a^{(p+3)/4} \pmod{p}$  and  $(\pm 2^{2n+1} a^{n+1})^2 \equiv 2^{(p-1)/2} a^{(p+3)/2} \equiv -a^{(p+3)/2} \pmod{p}$ . Since  $a$  is a quadratic residue,  $a^{(p-1)/2} \equiv 1 \pmod{p}$ , hence  $a^{(p-1)/4} \equiv \pm 1 \pmod{p}$ . But then  $\pm a^{(p+3)/4} \equiv a \pmod{p}$ .

**Question 5.** Show there are infinitely many primes of the form  $4k + 1$ .

Suppose there are finitely many such primes, say,  $p_1, p_2, \dots, p_k$ . Consider  $N = 4(p_1 \cdots p_k)^2 + 1$ , and let  $q$  be a prime divisor of  $N$ . Then  $q \neq p_i$  for any  $i$ , but  $N \equiv 0 \pmod{q}$ ; hence,  $4(p_1 \cdots p_k)^2 \equiv -1 \pmod{q}$ . Therefore,  $(-1|q) = 1$  which implies  $q \equiv 1 \pmod{4}$ , a contradiction. Therefore, there are infinitely primes which are 1 modulo 4.

**Question 6.** Show there are infinitely many primes of the following forms (a)  $8k + 3$ , (b)  $8k + 5$ , and (c)  $8k + 7$ . [Hint: For each part, assume there are only finitely many primes  $p_1, p_2, \dots, p_k$  of the required form. For (a), consider  $(p_1 \cdots p_k)^2 + 2$ ; for (b), consider  $(p_1 \cdots p_k)^2 + 4$ ; for (c), consider  $(4p_1 \cdots p_k)^2 - 2$ . Use what you know about  $(-1|p)$  and  $(2|p)$ .]

(a) Let  $N = (p_1 \cdots p_k)^2 + 2$ ; then  $N \equiv 3 \pmod{8}$ . Note that the product of two integers which are 1 mod 8 is again 1 mod 8. Therefore,  $N$  has an odd prime divisor  $q \not\equiv 1 \pmod{8}$ . Since  $N \equiv 0 \pmod{q}$ , we have that  $(p_1 \cdots p_k)^2 \equiv -2 \pmod{q}$ , hence  $(-2|q) = 1$ . Therefore,  $q \equiv 1$  or  $3 \pmod{8}$ . But we have excluded the case  $q \equiv 1 \pmod{8}$ . But we easily see that  $q \neq p_i$  for all  $i$ . We have, therefore, reached a contradiction.

(b) Let  $N = (p_1 \cdots p_k)^2 + 4$ ; then  $N \equiv 5 \pmod{8}$ . As before, there is an odd prime divisor  $q \not\equiv 1 \pmod{8}$  and  $q \neq p_i$  for any  $i$ . But then  $(p_1 \cdots p_k)^2 \equiv -4 \pmod{q}$ . Since 4 is a quadratic residue, so  $-1$  must also be a quadratic residue. Hence  $q \equiv 1 \pmod{4}$ . But  $q \not\equiv 1 \pmod{8}$ , hence  $q \equiv 5 \pmod{8}$ . We have reached our contradiction.

(c) Let  $N = (4p_1 \cdots p_k)^2 - 2$ . Then  $N/2 \equiv 7 \pmod{8}$ . and must have an odd prime divisor  $q \not\equiv 1 \pmod{8}$ . We have that  $2 \equiv (4p_1 \cdots p_k)^2 \pmod{q}$ , so  $(2 | q) = 1$  and  $q \equiv \pm 1 \pmod{8}$ . Hence,  $q \equiv -1 \pmod{8}$ , and we again reach a contradiction.

**Question 7.** Show the following. (a) If  $p = 4k + 1$  is a prime, then there is an integer  $x$  such that  $mp = 1 + x^2$  where  $0 < m < p$ . (b) If  $p$  is an odd prime, then there are integers  $x$  and  $y$  such that  $1 + x^2 + y^2 = mp$  where again  $0 < m < p$ .

(a) Since  $p \equiv 1 \pmod{4}$ , we know that  $-1$  is a quadratic residue of  $p$  and hence is one of  $1^2, 2^2, \dots, [(p-1)/2]^2$ , say,  $x^2$ . But,  $0 < 1 + x^2 < 1 + (p/2)^2 < p^2$ .

(b) The  $(p+1)/2$  numbers  $x : 0 \leq x \leq (p-1)/2$  are incongruent. Also, the  $(p+1)/2$  numbers  $-1 - y^2 : 0 \leq y \leq (p-1)/2$  are incongruent. The cardinalities of these two sets sum to  $p+1$ ; as there are only  $p$  residues modulo  $p$ , one must reside in both sets. Additionally,  $0 < 1 + x^2 + y^2 < 1 + 2(p/2)^2 < p^2$ .

**Question 8.** Determine those primes for which 7 is a quadratic residue.

By quadratic reciprocity, we have that  $(7 | p) = (-1)^{(p-1)/2} (p | 7)$ . Suppose first that  $p \equiv 1 \pmod{4}$ : if  $p \equiv 1 \pmod{7}$ , then  $p \equiv 1 \pmod{28}$ ; if  $p \equiv 2 \pmod{7}$ , then  $p \equiv 9 \pmod{28}$ ; if  $p \equiv 4 \pmod{7}$ , then  $p \equiv -3 \pmod{28}$ . Suppose next that  $p \equiv 3 \pmod{4}$ : if  $p \equiv 3 \pmod{7}$ , then  $p \equiv 3 \pmod{28}$ ; if  $p \equiv 5 \pmod{7}$ , then  $p \equiv -9 \pmod{28}$ ; if  $p \equiv 6 \pmod{7}$ , then  $p \equiv -1 \pmod{28}$ . We have, therefore, shown the following

$$\left(\frac{7}{p}\right) = \begin{cases} 1 & \text{if } p \equiv \pm 1, \pm 3, \pm 9 \pmod{28}, \\ -1 & \text{if } p \equiv \pm 5, \pm 7, \pm 11, \pm 13 \pmod{28}. \end{cases}$$

Let  $a$  and  $n$  be positive integers with  $n$  odd, and let  $n = p_1^{e_1} \cdots p_k^{e_k}$  be the prime power factorization of  $n$ . The Jacobi symbol is defined as  $(a | n) = (a | p_1)^{e_1} \cdots (a | p_k)^{e_k}$ .

**Question 9.** Prove the following properties of the Jacobi symbol. (a) If  $a \equiv b \pmod{n}$ , then  $(a | n) = (b | n)$ ; (b)  $(ab | n) = (a | n)(b | n)$ ; (c)  $(-1 | n) = (-1)^{(n-1)/2}$ ; (d)  $(2 | n) = (-1)^{(n^2-1)/8}$ . [Hint: Use the fact that  $(1 + (x-1))(1 + (y-1)) = xy$ .]

(a) We know that if  $a \equiv b \pmod{p}$ , then  $(a | p) = (b | p)$ . Hence,

$$\left(\frac{a}{n}\right) = \prod_i \left(\frac{a}{p_i}\right)^{e_i} = \prod_i \left(\frac{b}{p_i}\right)^{e_i} = \left(\frac{b}{n}\right).$$

(b) By the totally multiplicative property of the Legendre symbol, we have

$$\left(\frac{ab}{n}\right) = \prod_i \left(\frac{ab}{p_i}\right)^{e_i} = \prod_i \left(\frac{a}{p_i}\right)^{e_i} \left(\frac{b}{p_i}\right)^{e_i} = \left(\prod_i \left(\frac{a}{p_i}\right)^{e_i}\right) \left(\prod_i \left(\frac{b}{p_i}\right)^{e_i}\right) = \left(\frac{a}{n}\right) \left(\frac{b}{n}\right).$$

(c) We have

$$\left(\frac{-1}{n}\right) = \prod_i \left(\frac{-1}{p_i}\right)^{e_i} = (-1)^{\frac{1}{2} \sum_i (p_i-1)e_i}.$$

An obvious induction using the hint implies that  $n = \prod_i (1 + (p_i - 1))^{e_i}$ . Furthermore,  $(1 + (p_i - 1))^{e_i} \equiv 1 + e_i(p_i - 1) \pmod{4}$  and  $(1 + (p_i - 1))^{e_i} (1 + (p_j - 1))^{e_j} \equiv 1 + e_i(p_i - 1) + e_j(p_j - 1) \pmod{4}$ . Another clear induction shows  $n = \prod_i (1 + (p_i - 1))^{e_i} \equiv 1 + \sum_i e_i(p_i - 1) \pmod{4}$ . Since then  $(n - 1)/2 \equiv \sum_i e_i(p_i - 1)/2 \pmod{2}$ , the result now follows.

(d) Similar reasoning as that used in part (c) yields

$$\left(\frac{2}{n}\right) = (-1)^{\frac{1}{8} \sum_i e_i(p_i^2 - 1)}.$$

As before,  $n^2 \equiv 1 + \sum_i e_i(p_i^2 - 1) \pmod{4}$ . The result follows as above.

**Question 10.** Prove quadratic reciprocity holds for the Jacobi symbol, i.e.,  $(n \mid m)(m \mid n) = (-1)^{(m-1)(n-1)/4}$ .

Let  $n = \prod_{i=1}^s p_i^{e_i}$  and  $m = \prod_{j=1}^t q_j^{f_j}$ . By the definition of the Jacobi symbol and the total multiplicativity of the Legendre symbol,

$$\left(\frac{m}{n}\right) \left(\frac{n}{m}\right) = \prod_{i=1}^s \prod_{j=1}^t \left[ \left(\frac{p_i}{q_j}\right) \left(\frac{q_j}{p_i}\right) \right]^{e_i f_j}.$$

Quadratic reciprocity now gives

$$\left(\frac{m}{n}\right) \left(\frac{n}{m}\right) = \prod_{i=1}^s \prod_{j=1}^t (-1)^{(p_i-1)(q_j-1)e_i f_j / 4} = (-1)^{\sum_{i=1}^s \sum_{j=1}^t e_i \frac{p_i-1}{2} f_j \frac{q_j-1}{2}} = (-1)^{(\sum_{i=1}^s e_i \frac{p_i-1}{2})(\sum_{j=1}^t f_j \frac{q_j-1}{2})}.$$

As in question 9, we have that

$$\begin{aligned} \sum_{i=1}^s e_i \frac{p_i-1}{2} &\equiv \frac{n-1}{2} \pmod{2}, \\ \sum_{j=1}^t f_j \frac{q_j-1}{2} &\equiv \frac{m-1}{2} \pmod{2}. \end{aligned}$$

Therefore,

$$\left(\frac{m}{n}\right) \left(\frac{n}{m}\right) = (-1)^{(n-1)(m-1)/4}.$$